GPUCSL/GPUCSL.v
@@ -32,9 +32,14 @@ Ltac ex_intros vs H :=
     | (?v, ?vs) => ex_intro v H; ex_intros vs H
   end.
 
-Infix "+C" := (Eplus) (at level 50, left associativity).
-Infix "*C" := (Emult) (at level 40, left associativity).
-Infix "-C" := (Esub) (at level 50, left associativity).
-Infix "<C" := (Blt) (at level 70).
-
+Infix "+C" := (Ebinop OP_plus) (at level 50, left associativity).
+Infix "*C" := (Ebinop OP_mult) (at level 40, left associativity).
+Infix "-C" := (Ebinop OP_sub) (at level 50, left associativity).
+Infix "<C" := (Bcomp OP_blt) (at level 55).
+Infix "==C" := (Bcomp OP_beq) (at level 55).
+Infix "/C" := (Ebinop OP_div) (at level 40, left associativity) : exp_scope.
+Infix "%C" := (Ebinop OP_mod) (at level 40, left associativity) : exp_scope.
+Infix "&&C" := (Bbool OP_and) (at level 57, left associativity) : exp_scope.
+Infix "||C" := (Bbool OP_or) (at level 58, left associativity) : exp_scope.
+Notation minC x y := (Ebinop OP_min x y).
 Notation Zn := Z.of_nat.
